fvi lore

Refinery/Term/Syntax/FreeVar.lean
@@ -1,1 +1,38 @@
---TODO: utilities for counting free variables, substituting and renaming up to free variables
+import Refinery.Term.Syntax.Basic
+
+namespace Refinery
+
+namespace Term
+
+variable {φ : Type u} {α : Type v}
+
+def fvi : Term φ α → ℕ
+  | .bv ix => ix + 1
+  | .op _ a => fvi a
+  | .let₁ a _ b => max (fvi a) (fvi b - 1)
+  | .let₂ a _ _ b => max (fvi a) (fvi b - 2)
+  | .unit => 0
+  | .pair a b => max (fvi a) (fvi b)
+  | .inl _ _ a => fvi a
+  | .inr _ _ b => fvi b
+  | .case a _ _ b c => max (fvi a) (max (fvi b - 1) (fvi c - 1))
+  | .abort _ a => fvi a
+  | .iter a _ _ b => max (fvi a) (fvi b - 1)
+  | .invalid => 0
+
+theorem Subst.eqOn_pred_eqOn_lift (σ σ' : Subst φ α) (k : ℕ)
+  : (∀n < k - 1, σ.get n = σ'.get n) → (∀n < k, σ.lift.get n = σ'.lift.get n)
+  := λh n hn => match n with | 0 => rfl | n + 1 => by simp only [Subst.get_lift_succ]; rw [h]; omega
+
+theorem eqOn_fvi {a : Term φ α} (σ σ' : Subst φ α) (h : ∀n < a.fvi, σ.get n = σ'.get n)
+  : a.subst σ = a.subst σ' := by induction a generalizing σ σ' with
+  | bv => apply h; simp [fvi]
+  | _ =>
+    simp only [fvi, lt_sup_iff, or_imp, forall_and] at h
+    (try casesm* _ ∧ _)
+    simp
+    repeat first | apply And.intro | apply_assumption | apply Subst.eqOn_pred_eqOn_lift
+
+end Term
+
+end Refinery
