Refinery/Term/Extrinsic/FreeVar.lean
@@ -1,0 +1,22 @@
+import Refinery.Term.Syntax.FreeVar
+import Refinery.Term.Extrinsic.Typing
+
+namespace Refinery
+
+namespace Term
+
+variable {φ : Type u} {α : Type v} {ε : Type w} [S : Signature φ α ε]
+
+theorem Deriv.fvi_le_length
+  {Γ : Ctx? α} {A : Ty α} {a : Term φ (Ty α)} (da : Γ ⊢ a : A) : a.fvi ≤ Γ.length := by
+  induction da with
+  | bv hΓ =>
+    have _ := hΓ.length_lt;
+    rw [fvi]; omega
+  | _ =>
+    try (
+      rename Ctx?.SSplit _ _ _ => hΓ;
+      have hΓl := hΓ.left_length.symm;
+      have hΓr := hΓ.right_length.symm
+    )
+    simp [fvi, *] at * <;> simp [*]
